Lampe/Lampe/Syntax/Builders.lean
@@ -9,11 +9,13 @@ import Lampe.Builtin.BigInt
 import Lampe.Builtin.Bit
 import Lampe.Builtin.Cmp
 import Lampe.Builtin.Field
+import Lampe.Builtin.Lens
 import Lampe.Builtin.Memory
 import Lampe.Builtin.Slice
 import Lampe.Builtin.Str
 import Lampe.Builtin.Struct
-import Lampe.Builtin.Lens
+import Lampe.Semantics.Env
+import Lampe.Semantics.Trait
 import Lampe.Syntax.Rules
 import Lampe.Syntax.State
 import Lampe.Syntax.Utils
@@ -495,6 +497,18 @@ def makeTraitDef [MonadUtil m] : Syntax → m (List $ TSyntax `command)
   let associatedTypesKindDecl ←
     `(abbrev $(makeTraitDefAssociatedTypesKindsIdent traitName) : List Kind := $assocTypeGenKinds)
   outputs := outputs.concat associatedTypesKindDecl
+
+  let traitHasImplDecl : TSyntax `command ← 
+    `(@[reducible] def $(makeTraitDefHasImplIdent traitName) 
+      (env : $(←``(Env)))
+      (traitGenerics : HList Kind.denote $(makeTraitDefGenericKindsIdent traitName))
+      (selfType : Tp) :=
+        $(←``(TraitResolvable)) env 
+        ⟨⟨$(Syntax.mkStrLit traitName.getId.toString), 
+          $(makeTraitDefGenericKindsIdent traitName), 
+          traitGenerics⟩, 
+        selfType⟩)
+  outputs := outputs.concat traitHasImplDecl
 
   for method in methods.getElems.toList do match method with
   | `(noir_trait_method|method $methName < $methGens,*> ( $params,* ) → $retType)
