stdlib/lampe/Stdlib/Array/Quicksort.lean
@@ -2,14 +2,12 @@ import «std-1.0.0-beta.12».Extracted.Array.Quicksort
 import «std-1.0.0-beta.12».Extracted.«std-1.0.0-beta.12»
 import Lampe
 
-namespace Lampe
-namespace Stdlib
+namespace Lampe.Stdlib.Array.Quicksort
 
 export «std-1.0.0-beta.12».Extracted (
   «std::array::quicksort::partition»
   «std::array::quicksort::quicksort_loop»
   «std::array::quicksort::quicksort»
-  Array.Quicksort.env
 )
 
 open «std-1.0.0-beta.12».Extracted
