stdlib/lampe/Stdlib/Convert.lean
@@ -2,8 +2,7 @@ import «std-1.0.0-beta.12».Extracted.Convert
 import «std-1.0.0-beta.12».Extracted.«std-1.0.0-beta.12»
 import Lampe
 
-namespace Lampe
-namespace Stdlib
+namespace Lampe.Stdlib.Convert
 
 export «std-1.0.0-beta.12».Extracted (
   «std::convert::AsPrimitive».«#genericKinds»
@@ -24,7 +23,6 @@ export «std-1.0.0-beta.12».Extracted (
   «std::convert::Into».into.«#inputs»
   «std::convert::Into».into.«#output»
   «std::convert::Into».into
-  Convert.env
 )
 
 open «std-1.0.0-beta.12».Extracted
