stdlib/lampe/Stdlib/Hash/Mod.lean
@@ -2,8 +2,7 @@ import «std-1.0.0-beta.12».Extracted.Hash.Mod
 import «std-1.0.0-beta.12».Extracted.«std-1.0.0-beta.12»
 import Lampe
 
-namespace Lampe
-namespace Stdlib
+namespace Lampe.Stdlib.Hash
 
 export «std-1.0.0-beta.12».Extracted (
   «std::hash::keccak::keccakf1600»
@@ -15,7 +14,6 @@ export «std-1.0.0-beta.12».Extracted (
   «std::hash::derive_generators»
   «std::hash::from_field_unsafe»
   «std::hash::assert_pedersen»
-  Hash.Mod.env
 )
 
 open «std-1.0.0-beta.12».Extracted
