stdlib/lampe/Stdlib/Hash/Poseidon2.lean
@@ -2,8 +2,7 @@ import «std-1.0.0-beta.12».Extracted.Hash.Poseidon2
 import «std-1.0.0-beta.12».Extracted.«std-1.0.0-beta.12»
 import Lampe
 
-namespace Lampe
-namespace Stdlib
+namespace Lampe.Stdlib.Hash.Poseidon2
 
 export «std-1.0.0-beta.12».Extracted (
   «std::hash::poseidon2::Poseidon2»
@@ -13,7 +12,6 @@ export «std-1.0.0-beta.12».Extracted (
   «std::hash::poseidon2::Poseidon2::absorb»
   «std::hash::poseidon2::Poseidon2::squeeze»
   «std::hash::poseidon2::Poseidon2::hash_internal»
-  Hash.Poseidon2.env
 )
 
 open «std-1.0.0-beta.12».Extracted
