stdlib/lampe/Stdlib/Lib.lean
@@ -2,8 +2,7 @@ import «std-1.0.0-beta.12».Extracted.Lib
 import «std-1.0.0-beta.12».Extracted.«std-1.0.0-beta.12»
 import Lampe
 
-namespace Lampe
-namespace Stdlib
+namespace Lampe.Stdlib.Lib
 
 export «std-1.0.0-beta.12».Extracted (
   «std::print_oracle»
@@ -16,7 +15,6 @@ export «std-1.0.0-beta.12».Extracted (
   «std::wrapping_mul»
   «std::tests::test_static_assert_custom_message»
   «std::tests::test_wrapping_mul»
-  Lib.env
 )
 
 open «std-1.0.0-beta.12».Extracted
