stdlib/lampe/Stdlib/Option.lean
@@ -1,9 +1,8 @@
-import «std-1.0.0-beta.12».Extracted.Option
 import «std-1.0.0-beta.12».Extracted.«std-1.0.0-beta.12»
+import Stdlib.Cmp
 import Lampe
 
-namespace Lampe
-namespace Stdlib
+namespace Lampe.Stdlib.Option
 
 export «std-1.0.0-beta.12».Extracted (
   «std::option::Option»
@@ -25,14 +24,15 @@ export «std-1.0.0-beta.12».Extracted (
   «std::option::Option::or_else»
   «std::option::Option::xor»
   «std::option::Option::flatten»
-  Option.env
 )
 
 open «std-1.0.0-beta.12».Extracted
+open Cmp.Ord
 
-namespace Option
+set_option Lampe.pp.Expr false
+set_option Lampe.pp.STHoare false
 
-/-- 
+/--
 Convert a Lean option into a Noir `std::option::Option`.
 
 We recommend providing the user with `std::option::Option`s at the boundary of the theorem for any
@@ -42,7 +42,7 @@ def fromOption {p t} : Option (t.denote p) -> («std::option::Option».tp h![t] 
 | none => (false, Tp.zero p t, ())
 | some val => (true, val, ())
 
-/-- 
+/--
 Convert a Noir `std::option::Option` into a Lean option.
 
 We recommend converting user-provided `std::option::Option`s from the user, and converting them
@@ -57,10 +57,10 @@ lemma fromOption_toOption_id : toOption (fromOption v) = v := by
   cases v <;> rfl
 
 @[simp]
-lemma option_fst_eq_toOption_isSome {p T} 
+lemma option_fst_eq_toOption_isSome {p T}
     {v : Tp.denote p $ «std::option::Option».tp h![T]}
   : Builtin.indexTpl v Builtin.Member.head = (toOption v).isSome := by
-  rcases v with ⟨_|_, _⟩ 
+  rcases v with ⟨_|_, _⟩
   all_goals rfl
 
 @[simp]
@@ -68,9 +68,9 @@ lemma option_snd_eq_toOption_get_of_isSome {p T}
     {v : Tp.denote p $ «std::option::Option».tp h![T]}
     (v_is_some : (toOption v).isSome = true)
   : Builtin.indexTpl v Builtin.Member.head.tail = (toOption v).get v_is_some := by
-  rcases v with ⟨_|_, _, _⟩ 
-  . contradiction
-  . rfl
+  rcases v with ⟨_|_, _, _⟩
+  · contradiction
+  · rfl
 
 lemma getD_map_of_isSome {α β} {f : α → β} {d : β} {o : Option α}
     (h : o.isSome)
@@ -79,12 +79,12 @@ lemma getD_map_of_isSome {α β} {f : α → β} {d : β} {o : Option α}
   rfl
 
 @[simp]
-lemma bind_def_of_isSome {α β} {v : Option α} {f : α → Option β} (v_is_some : v.isSome = true) 
-  : v >>= f = f (v.get v_is_some) := by  
+lemma bind_def_of_isSome {α β} {v : Option α} {f : α → Option β} (v_is_some : v.isSome = true)
+  : v >>= f = f (v.get v_is_some) := by
   rcases (Option.isSome_iff_exists.mp v_is_some) with ⟨_, rfl⟩
   simp_all
 
-theorem none_spec {p T} : STHoare p env ⟦⟧ («std::option::Option::none».call h![T] h![]) 
+theorem none_spec {p T} : STHoare p env ⟦⟧ («std::option::Option::none».call h![T] h![])
     (fun v => v = fromOption none) := by
   enter_decl
   steps
@@ -98,8 +98,8 @@ theorem some_spec {p T v} : STHoare p env ⟦⟧ («std::option::Option::some».
   subst_vars
   rfl
 
-theorem is_none_spec {p T v} : STHoare p env ⟦⟧ 
-    («std::option::Option::is_none».call h![T] h![v]) 
+theorem is_none_spec {p T v} : STHoare p env ⟦⟧
+    («std::option::Option::is_none».call h![T] h![v])
     (fun r => r = (toOption v).isNone) := by
   enter_decl
   steps
@@ -107,16 +107,16 @@ theorem is_none_spec {p T v} : STHoare p env ⟦⟧
   simp
   exact ()
 
-theorem is_some_spec {p T v} : STHoare p env ⟦⟧ 
-    («std::option::Option::is_some».call h![T] h![v]) 
+theorem is_some_spec {p T v} : STHoare p env ⟦⟧
+    («std::option::Option::is_some».call h![T] h![v])
     (fun r => r = (toOption v).isSome) := by
   enter_decl
   steps
   subst_vars
   simp
 
-theorem unwrap_spec {p T v} : STHoare p env ⟦⟧ 
-    («std::option::Option::unwrap».call h![T] h![v]) 
+theorem unwrap_spec {p T v} : STHoare p env ⟦⟧
+    («std::option::Option::unwrap».call h![T] h![v])
     (fun r => ∃h, r = (toOption v).get h) := by
   enter_decl
   steps
@@ -126,18 +126,18 @@ theorem unwrap_spec {p T v} : STHoare p env ⟦⟧
   subst_vars
   rename Tp.denote p («std::option::Option».tp _) => h
   rcases h with ⟨(_|_), _, _⟩
-  . contradiction
-  . rfl
+  · contradiction
+  · rfl
 
-theorem map_none_spec {p T U E f v} 
+theorem map_none_spec {p T U E f v}
     (v_is_none : (toOption v).isNone)
-  : STHoare p env ⟦⟧ 
-    («std::option::Option::map».call h![T, U, E] h![v, f]) 
+  : STHoare p env ⟦⟧
+    («std::option::Option::map».call h![T, U, E] h![v, f])
     (fun r => r = fromOption none) := by
   enter_decl
   steps
   apply STHoare.ite_intro_of_false
-  . simp_all
+  · simp_all
 
   steps [none_spec]
   simp_all
@@ -152,7 +152,7 @@ theorem map_some_spec {p T U E f fb v P Q}
   enter_decl
   steps
   apply STHoare.ite_intro_of_true
-  . simp_all
+  · simp_all
 
   steps
   simp only [option_snd_eq_toOption_get_of_isSome v_is_some]
@@ -163,15 +163,15 @@ theorem map_some_spec {p T U E f fb v P Q}
 theorem map_pure_spec {p T U E P f fb v}
     {f_emb : T.denote p → U.denote p}
     (h_f : ∀arg, STHoare p env P (fb h![arg]) (fun r => r = f_emb arg ⋆ P))
-  : STHoare p env 
+  : STHoare p env
     (P ⋆ [λf ↦ fb])
-    («std::option::Option::map».call h![T, U, E] h![v, f]) 
+    («std::option::Option::map».call h![T, U, E] h![v, f])
     (fun r => r = fromOption ((toOption v).map f_emb) ⋆ P) := by
   by_cases h : (toOption v).isSome = true
-  . steps [map_some_spec h (h_f _)]
+  · steps [map_some_spec h (h_f _)]
     subst_vars
     simp only [←Option.map_some, Option.some_get]
-  . steps [map_none_spec]
+  · steps [map_none_spec]
     all_goals simp_all
 
 theorem map_or_none_spec {p T U E v default f}
@@ -182,8 +182,8 @@ theorem map_or_none_spec {p T U E v default f}
   enter_decl
   steps
   apply STHoare.ite_intro_of_false
-  . simp_all
-  
+  · simp_all
+
   steps
   simp_all
 
@@ -197,7 +197,7 @@ theorem map_or_some_spec {p T U E v f fb default P Q}
   enter_decl
   steps
   apply STHoare.ite_intro_of_true
-  . simp_all
+  · simp_all
 
   steps
   simp only [option_snd_eq_toOption_get_of_isSome v_is_some]
@@ -211,10 +211,10 @@ theorem map_or_pure_spec {p T U E P v f fb default}
     («std::option::Option::map_or».call h![T, U, E] h![v, default, f])
     (fun r => r = ((toOption v).map f_emb).getD default ⋆ P) := by
   by_cases h : (toOption v).isSome = true
-  . steps [map_or_some_spec (E := E) h (h_f _)]
+  · steps [map_or_some_spec (E := E) h (h_f _)]
     subst_vars
     rw [getD_map_of_isSome (f := f_emb) h]
-  . steps [map_or_none_spec]
+  · steps [map_or_none_spec]
     all_goals simp_all
 
 theorem map_or_else_none_spec {p T U E1 E2 P Q v default default_b func}
@@ -227,7 +227,7 @@ theorem map_or_else_none_spec {p T U E1 E2 P Q v default default_b func}
   enter_decl
   steps
   apply STHoare.ite_intro_of_false
-  . simp_all
+  · simp_all
 
   steps [STHoare.callLambda_intro (hlam := default_f)]
 
@@ -241,7 +241,7 @@ theorem map_or_else_some_spec {p T U E1 E2 P Q v default func func_b}
   enter_decl
   steps
   apply STHoare.ite_intro_of_true
-  . simp_all
+  · simp_all
 
   steps
   simp only [option_snd_eq_toOption_get_of_isSome v_is_some]
@@ -257,10 +257,10 @@ theorem map_or_else_pure_spec {p T U E1 E2 P v default default_b func func_b}
     («std::option::Option::map_or_else».call h![T, U, E1, E2] h![v, default, func])
     (fun r => r = ((toOption v).map func_emb).getD default_emb ⋆ P) := by
   by_cases h : (toOption v).isSome = true
-  . steps [map_or_else_some_spec (E1 := E1) (E2 := E2) h (func_f _)]
+  · steps [map_or_else_some_spec (E1 := E1) (E2 := E2) h (func_f _)]
     subst_vars
     rw [getD_map_of_isSome (f := func_emb) h]
-  . have h : (toOption v).isNone := by 
+  · have h : (toOption v).isNone := by
       simp_all
     steps [map_or_else_none_spec (E1 := E1) (E2 := E2) h default_f]
     subst_vars
@@ -273,23 +273,23 @@ theorem and_spec {p T v w}
   enter_decl
   steps [is_none_spec]
   apply STHoare.ite_intro
-  . intro cond
+  · intro cond
     steps [none_spec]
     simp_all
-  . intro cond
+  · intro cond
     steps
     simp_all
 
 theorem and_then_none_spec {p T U E self f}
     (self_is_none : (toOption self).isNone)
-  : STHoare p env ⟦⟧ 
+  : STHoare p env ⟦⟧
     («std::option::Option::and_then».call h![T, U, E] h![self, f])
     (fun r => r = fromOption none) := by
   enter_decl
   steps
   apply STHoare.ite_intro_of_false
-  . simp_all
-  
+  · simp_all
+
   steps [none_spec]
   simp_all
 
@@ -303,8 +303,8 @@ theorem and_then_some_spec {p T U E P Q self f fb}
   enter_decl
   steps
   apply STHoare.ite_intro_of_true
-  . simp_all
-  
+  · simp_all
+
   steps
   simp [option_snd_eq_toOption_get_of_isSome self_is_some]
   steps [STHoare.callLambda_intro (hlam := f_lam)]
@@ -317,10 +317,10 @@ theorem and_then_pure_spec {p T U E P self f fb}
     («std::option::Option::and_then».call h![T, U, E] h![self, f])
     (fun r => r = ((toOption self).map f_emb).getD (fromOption none) ⋆ P) := by
   by_cases h : (toOption self).isSome = true
-  . steps [and_then_some_spec (E := E) h (f_f _)]
+  · steps [and_then_some_spec (E := E) h (f_f _)]
     subst_vars
     rw [getD_map_of_isSome h]
-  . have h : (toOption self).isNone := by simp_all
+  · have h : (toOption self).isNone := by simp_all
     steps [and_then_none_spec (E := E) h]
     simp_all
 
@@ -331,12 +331,12 @@ theorem or_spec {p T self default}
   enter_decl
   steps
   apply STHoare.ite_intro
-  . intro cond
+  · intro cond
     rw [option_fst_eq_toOption_isSome] at cond
     steps
     subst_vars
     simp_all
-  . intro cond
+  · intro cond
     rw [option_fst_eq_toOption_isSome] at cond
     simp_all only [Option.isSome_eq_false_iff, Option.isNone_iff_eq_none, Option.isSome_none,
                    Bool.false_eq_true, ↓reduceIte]
@@ -346,14 +346,14 @@ theorem or_spec {p T self default}
 theorem or_else_none_spec {p T E P Q self default default_b}
     (self_is_none : (toOption self).isNone)
     (default_f : STHoare p env P (default_b h![]) Q)
-  : STHoare p env 
+  : STHoare p env
     (P ⋆ [λdefault ↦ default_b])
     («std::option::Option::or_else».call h![T, E] h![self, default])
     (fun r => Q r ⋆ [λdefault ↦ default_b]) := by
   enter_decl
   steps
   apply STHoare.ite_intro_of_false
-  . simp_all
+  · simp_all
 
   steps [STHoare.callLambda_intro (hlam := default_f)]
 
@@ -365,7 +365,7 @@ theorem or_else_some_spec {p T E self default}
   enter_decl
   steps
   apply STHoare.ite_intro_of_true
-  . simp_all
+  · simp_all
 
   steps
   simp_all
@@ -381,7 +381,7 @@ theorem or_else_pure_spec {p T E P self default default_b}
   . steps [or_else_some_spec h]
     subst_vars
     simp_all
-  . have h : (toOption self).isNone := by simp_all
+  · have h : (toOption self).isNone := by simp_all
     steps [or_else_none_spec (E := E) h default_f]
     subst_vars
     simp_all
@@ -389,8 +389,8 @@ theorem or_else_pure_spec {p T E P self default default_b}
 theorem xor_spec {p T self other}
   : STHoare p env ⟦⟧
     («std::option::Option::xor».call h![T] h![self, other])
-    (fun r => r = if (toOption self).isSome then 
-        if (toOption other).isSome then fromOption none else self 
+    (fun r => r = if (toOption self).isSome then
+        if (toOption other).isSome then fromOption none else self
       else if (toOption other).isSome then
         other
       else
@@ -399,35 +399,35 @@ theorem xor_spec {p T self other}
   enter_decl
   steps
   apply STHoare.ite_intro
-  . intros
+  · intros
     steps
     apply STHoare.ite_intro
-    . intros
+    · intros
       steps [none_spec]
       simp_all
-    . intros
+    · intros
       steps
       simp_all
-  . intros
+  · intros
     steps
     apply STHoare.ite_intro
-    . intros
+    · intros
       steps
       simp_all
-    . intros
+    · intros
       steps [none_spec]
       simp_all
 
 theorem filter_none_spec {p T E self pred}
     (self_is_none : (toOption self).isNone)
-  : STHoare p env ⟦⟧ 
+  : STHoare p env ⟦⟧
     («std::option::Option::filter».call h![T, E] h![self, pred])
     (fun r => r = fromOption none) := by
   enter_decl
   steps
   rw [option_fst_eq_toOption_isSome]
   apply STHoare.ite_intro_of_false
-  . simp_all
+  · simp_all
 
   steps [none_spec]
   simp_all
@@ -443,19 +443,19 @@ theorem filter_some_spec {p T E P Q self pred pred_b}
   steps
   rw [option_fst_eq_toOption_isSome]
   apply STHoare.ite_intro_of_true
-  . simp_all
+  · simp_all
 
   steps
   simp_all only [option_snd_eq_toOption_get_of_isSome]
   steps [STHoare.callLambda_intro (hlam := pred_f)]
 
   apply STHoare.ite_intro
-  . intros
+  · intros
     steps unsafe
     subst_vars
     simp_all
-      
-  . intros
+
+  · intros
     steps [none_spec]
     subst_vars
     sl unsafe
@@ -469,7 +469,7 @@ theorem flatten_spec {p T opt}
   steps
   rw [option_fst_eq_toOption_isSome]
   apply STHoare.ite_intro
-  . intros
+  · intros
     steps
     subst_vars
     rw [option_snd_eq_toOption_get_of_isSome]
@@ -477,15 +477,189 @@ theorem flatten_spec {p T opt}
     simp_all
     apply Option.get_eq_getD
 
-  . intros
+  · intros
     steps [none_spec]
     subst_vars
     simp_all
 
-theorem default_spec {p T} : STHoare p env ⟦⟧ 
+set_option maxRecDepth 2000 in
+theorem default_spec {p T}
+  : STHoare p env ⟦⟧
     («std::default::Default».default h![] («std::option::Option».tp h![T]) h![] h![] h![])
     (fun r => r = fromOption none) := by
   resolve_trait
   steps [none_spec]
   simp_all
-    
+
+set_option maxRecDepth 2000 in
+theorem eq_spec {p T self other P Q}
+    {t_eq : «std::cmp::Eq».hasImpl env h![] T}
+    {eq_f : (h_self : (toOption self).isSome)
+          → (h_other : (toOption other).isSome)
+          → STHoare p env P
+            («std::cmp::Eq».eq h![] T h![] h![]
+              h![(toOption self).get h_self, (toOption other).get h_other])
+            Q}
+  : STHoare p env P
+    («std::cmp::Eq».eq h![] («std::option::Option».tp h![T]) h![] h![] h![self, other])
+    (fun r => if h : (toOption self).isSome ∧ (toOption other).isSome then
+        Q r else (r = ((toOption self).isSome == (toOption other).isSome))) := by
+  resolve_trait
+  steps
+  · exact ()
+  apply STHoare.ite_intro
+  · simp only [option_fst_eq_toOption_isSome, decide_eq_true_eq, dite_eq_ite]
+    intro hp
+    steps
+    apply STHoare.ite_intro
+    · simp only [option_fst_eq_toOption_isSome, decide_eq_true_eq, dite_eq_ite]
+      intro hs
+      rw [hs, Eq.comm] at hp
+      steps
+      simp only [option_snd_eq_toOption_get_of_isSome, *]
+      steps [eq_f hs hp]
+    · simp only [option_fst_eq_toOption_isSome, decide_eq_true_eq, dite_eq_ite]
+      intro hp
+      simp_all
+      steps
+      assumption
+  · simp only [option_fst_eq_toOption_isSome, decide_eq_false_iff_not, dite_eq_ite]
+    intro hp
+    split
+    · rename_i hh
+      rcases hh
+      simp_all
+    · steps
+      subst_vars
+      rw [Eq.comm, beq_eq_false_iff_ne]
+      assumption
+
+theorem eq_spec_pure {p T self other}
+    {t_eq : «std::cmp::Eq».hasImpl env h![] T}
+    {eq_emb : T.denote p → T.denote p → Prop}
+    (h_eq : ∀a b, STHoare p env ⟦⟧
+      («std::cmp::Eq».eq h![] T h![] h![] h![a, b])
+      (fun r : Bool => r = eq_emb a b))
+  : STHoare p env ⟦⟧
+    («std::cmp::Eq».eq h![] («std::option::Option».tp h![T]) h![] h![] h![self, other])
+    (fun r : Bool => r = Option.Rel eq_emb (toOption self) (toOption other)) := by
+  apply STHoare.consequence_frame
+  apply eq_spec
+  case t_eq => assumption
+  case eq_f =>
+    intros
+    simp only [←option_snd_eq_toOption_get_of_isSome]
+    apply h_eq
+  case h_ent => sl
+  case q_ent =>
+    intros
+    simp only [SL.dite_lift_lift]
+    sl
+    rename_i hp
+    split at hp
+    · casesm _∧_
+      rename_i hs ho
+      simp only [hp, option_snd_eq_toOption_get_of_isSome, *]
+      conv =>
+        rhs
+        congr
+        · skip
+        · rw [←Option.some_get hs]
+        · rw [←Option.some_get ho]
+      simp only [Option.rel_some_some]
+    · generalize toOption self = self at *
+      generalize toOption other = other at *
+      simp_all only [eq_iff_iff, not_and, Bool.not_eq_true, Option.isSome_eq_false_iff,
+        Option.isNone_iff_eq_none, beq_iff_eq]
+      apply Iff.intro
+      · intro hp
+        have : self.isSome = false := by
+          by_contra
+          simp_all
+        have : self = none := by simp_all
+        have : other = none := by simp_all
+        simp only [*, Option.rel_none_none]
+      · rintro (_ | _) <;> simp_all
+
+set_option maxRecDepth 2000 in
+theorem hash_spec {p T H self P Q R}
+    {state : Tp.denote p $ Tp.ref H}
+    {t_hash : «std::hash::Hash».hasImpl env h![] T}
+    {t_hash_f : (h_self : (toOption self).isSome) → STHoare p env Q
+      («std::hash::Hash».hash h![] T h![] h![H] h![(toOption self).get h_self, state]) fun _ => R}
+    {bool_hash : «std::hash::Hash».hasImpl env h![] Tp.bool}
+    {bool_hash_f : STHoare p env P
+      («std::hash::Hash».hash h![] Tp.bool h![] h![H] h![(toOption self).isSome, state]) fun _ => Q}
+  : STHoare p env P
+    («std::hash::Hash».hash h![] («std::option::Option».tp h![T]) h![] h![H] h![self, state])
+    (fun _ => if (toOption self).isSome then R else Q) := by
+  resolve_trait
+  steps
+
+  step_as (P) (fun _ => Q)
+  · rw [option_fst_eq_toOption_isSome]
+    steps [bool_hash_f]
+  · steps
+    apply STHoare.ite_intro
+    · simp_all only [option_fst_eq_toOption_isSome]
+      intros
+      steps
+      rw [option_snd_eq_toOption_get_of_isSome]
+      rename_i a
+      steps [t_hash_f a]
+
+    · simp only [option_fst_eq_toOption_isSome, Option.isSome_eq_false_iff,
+        Option.isNone_iff_eq_none]
+      intro
+      simp_all only [Option.isSome_none, Bool.false_eq_true, IsEmpty.forall_iff, ↓reduceIte]
+      steps
+
+set_option maxRecDepth 2000 in
+theorem cmp_spec {p T self other P Q}
+    {t_ord : «std::cmp::Ord».hasImpl env h![] T}
+    {t_ord_f : (h_self : (toOption self).isSome)
+             → (h_other : (toOption other).isSome)
+             → STHoare p env P
+               («std::cmp::Ord».cmp h![] T h![] h![]
+                h![(toOption self).get h_self, (toOption other).get h_other])
+               Q}
+  : STHoare p env P
+    («std::cmp::Ord».cmp h![] («std::option::Option».tp h![T]) h![] h![] h![self, other])
+    (fun r => if (toOption self).isSome then
+      if (toOption other).isSome then Q r else r = fromOrdering .gt
+    else if (toOption other).isSome then r = fromOrdering .lt else
+      r = fromOrdering .eq) := by
+  resolve_trait
+  steps
+  rw [option_fst_eq_toOption_isSome]
+  apply STHoare.ite_intro
+  · intro s_some
+    steps
+    rw [option_fst_eq_toOption_isSome]
+    apply STHoare.ite_intro
+    · intro o_some
+      steps
+      rw [option_snd_eq_toOption_get_of_isSome o_some, option_snd_eq_toOption_get_of_isSome s_some]
+      steps [t_ord_f s_some o_some]
+      simp_all only [forall_true_left, ↓reduceIte]
+      sl
+    · intro o_none
+      steps
+      conv => rhs; simp [s_some, o_none]
+      steps [greater_spec]
+      simp_all
+  · intro s_none
+    steps
+    rw [option_fst_eq_toOption_isSome]
+    apply STHoare.ite_intro
+    · intro o_some
+      steps
+      conv => rhs; simp [s_none, o_some]
+      steps [less_spec]
+      simp_all
+    · intro o_none
+      steps
+      conv => rhs; simp [s_none, o_none]
+      steps [equal_spec]
+      simp_all
+
