stdlib/lampe/Stdlib/Stdlib.lean
@@ -25,7 +25,6 @@ import Stdlib.String
 
 import «std-1.0.0-beta.12».Extracted.«std-1.0.0-beta.12»
 
-namespace Lampe
-namespace Stdlib
+namespace Lampe.Stdlib
 
 export «std-1.0.0-beta.12».Extracted (env)
