stdlib/lampe/Stdlib/String.lean
@@ -2,12 +2,10 @@ import «std-1.0.0-beta.12».Extracted.String
 import «std-1.0.0-beta.12».Extracted.«std-1.0.0-beta.12»
 import Lampe
 
-namespace Lampe
-namespace Stdlib
+namespace Lampe.Stdlib.String
 
 export «std-1.0.0-beta.12».Extracted (
   «std::string::as_bytes_vec»
-  String.env
 )
 
 open «std-1.0.0-beta.12».Extracted
